# **Factoring Polynomials**

## **Difference of Square**

Use to factor a **quadratic binomial** equation
in the form of ($a^2-c^2$) where each term could be
of any degree **less-than or equal degree 2**.

$a^2 - c^2 = (a + c)(a - c)$

**Example:**

$
4x^2 - 25 \\
a \implies{\sqrt{4x^2} = 2x} \\
c \implies{\sqrt{25} = 5} \\
= (2x + 5)(2x - 5)
$

**Proof**

$
\begin{align}
&= (a + c)(a - c) \\
&= a^2 + ac - ac - c^2 \\
&= a^2 + \cancel{ac - ac} - c^2 \\
&= a^2 - c^2
\end{align}
$

## **Difference of Square for non-prefect square binomials**

To factor out difference of square with non-prefect 
square terms, we need to factor out a term/constant
where the inner binomial terms have will have
perfect square terms.

**Example**

$
\begin{align}
&= 45x^2 - 125 \\
&= 5(9x^2 - 25) \\
&= 5(3x + 5)(3x - 5)
\end{align}
$

Here 45 and 125 are not perfect squares so we factor 
them out with 5 to make the inner binomial have perfect
square terms.